Launchbury/CorrectnessResourced.thy
@@ -111,13 +111,13 @@ case (Variable \<Gamma> x e L \<Delta> z)
 
   have "\<N>\<lbrace>\<Gamma>\<rbrace>\<rho> = \<N>\<lbrace>(x,e) # delete x \<Gamma>\<rbrace>\<rho>"
     by (rule HSem_reorder[OF map_of_delete_insert[symmetric, OF Variable(1)]])
-  also have "\<dots> = (\<mu> \<rho>'. (\<rho> f++\<^bsub>(domA (delete x \<Gamma>))\<^esub> (\<N>\<lbrace>delete x \<Gamma>\<rbrace>\<rho>'))( x := \<N>\<lbrakk> e \<rbrakk>\<^bsub>\<rho>'\<^esub>))"
+  also have "\<dots> = (\<mu> \<rho>'. (\<rho> ++\<^bsub>(domA (delete x \<Gamma>))\<^esub> (\<N>\<lbrace>delete x \<Gamma>\<rbrace>\<rho>'))( x := \<N>\<lbrakk> e \<rbrakk>\<^bsub>\<rho>'\<^esub>))"
     by (rule iterative_HSem, simp)
-  also have "\<dots> = (\<mu> \<rho>'. (\<rho> f++\<^bsub>(domA (delete x \<Gamma>))\<^esub> (\<N>\<lbrace>delete x \<Gamma>\<rbrace>\<rho>'))( x := \<N>\<lbrakk> e \<rbrakk>\<^bsub>\<N>\<lbrace>delete x \<Gamma>\<rbrace>\<rho>'\<^esub>))"
+  also have "\<dots> = (\<mu> \<rho>'. (\<rho> ++\<^bsub>(domA (delete x \<Gamma>))\<^esub> (\<N>\<lbrace>delete x \<Gamma>\<rbrace>\<rho>'))( x := \<N>\<lbrakk> e \<rbrakk>\<^bsub>\<N>\<lbrace>delete x \<Gamma>\<rbrace>\<rho>'\<^esub>))"
     by (rule iterative_HSem', simp)
   finally
   have "(\<N>\<lbrace>\<Gamma>\<rbrace>\<rho>)f|` (- ?new) \<sqsubseteq> (...) f|` (- ?new)" by (rule ssubst) (rule below_refl)
-  also have "\<dots> \<sqsubseteq> (\<mu> \<rho>'. (\<rho> f++\<^bsub>domA \<Delta>\<^esub> (\<N>\<lbrace>\<Delta>\<rbrace>\<rho>'))( x := \<N>\<lbrakk> z \<rbrakk>\<^bsub>\<N>\<lbrace>\<Delta>\<rbrace>\<rho>'\<^esub>)) f|` (- ?new)"
+  also have "\<dots> \<sqsubseteq> (\<mu> \<rho>'. (\<rho> ++\<^bsub>domA \<Delta>\<^esub> (\<N>\<lbrace>\<Delta>\<rbrace>\<rho>'))( x := \<N>\<lbrakk> z \<rbrakk>\<^bsub>\<N>\<lbrace>\<Delta>\<rbrace>\<rho>'\<^esub>)) f|` (- ?new)"
   proof (induction rule: parallel_fix_ind[where P ="\<lambda> x y. x f|` (- ?new) \<sqsubseteq> y f|` (- ?new)"])
     case 1 show ?case by simp
   next
@@ -132,9 +132,9 @@ case (Variable \<Gamma> x e L \<Delta> z)
        and "(\<N>\<lbrace>delete x \<Gamma>\<rbrace>\<sigma>) f|` domA (delete x \<Gamma>) \<sqsubseteq> (\<N>\<lbrace>\<Delta>\<rbrace>\<sigma>') f|` domA (delete x \<Gamma>)".
     thus ?case
       using subset
-      by (auto intro!: fun_belowI simp add: lookup_fun_merge_eq  lookup_fmap_restr_eq elim: fmap_restr_belowD)
+      by (auto intro!: fun_belowI simp add: lookup_override_on_eq  lookup_fmap_restr_eq elim: fmap_restr_belowD)
   qed
-  also have "\<dots> = (\<mu> \<rho>'. (\<rho> f++\<^bsub>domA \<Delta>\<^esub> (\<N>\<lbrace>\<Delta>\<rbrace>\<rho>'))( x := \<N>\<lbrakk> z \<rbrakk>\<^bsub>\<rho>'\<^esub>)) f|` (-?new)"
+  also have "\<dots> = (\<mu> \<rho>'. (\<rho> ++\<^bsub>domA \<Delta>\<^esub> (\<N>\<lbrace>\<Delta>\<rbrace>\<rho>'))( x := \<N>\<lbrakk> z \<rbrakk>\<^bsub>\<rho>'\<^esub>)) f|` (-?new)"
     by (rule arg_cong[OF iterative_HSem'[symmetric], OF `x \<notin> domA \<Delta>`])
   also have "\<dots> = (\<N>\<lbrace>(x,z) # \<Delta>\<rbrace>\<rho>)  f|` (-?new)"
     by (rule arg_cong[OF iterative_HSem[symmetric], OF `x \<notin> domA \<Delta>`])
